Remove nongeneric "symbol" terms.

Term.v
@@ -15,7 +15,7 @@ Create HintDb Term.
 (** Definitions *)
 Inductive Ty : Set :=
   TyBase
-| TyPair : Ty -> Ty -> Ty
+(* | TyPair : Ty -> Ty -> Ty *)
 | TyArr : Ty -> Ty -> Ty
 (* | TyAny : Ty *)
 | TyList : Ty -> Ty.
@@ -24,19 +24,20 @@ Inductive Ty : Set :=
 Inductive Term : Set :=
   TmConst
 | TmVar (x : nat) : Term
-| TmPair : Term -> Term -> Term
-| TmProj : bool -> Term -> Term
+(* | TmPair : Term -> Term -> Term
+| TmProj : bool -> Term -> Term *)
 | TmAbs : Term -> Term
 | TmApp : Term -> Term -> Term
-| TmNull : Term
+(* | TmNull : Term *)
 | TmSingle : Term -> Term
-| TmUnion : Term -> Term -> Term
+(* | TmUnion : Term -> Term -> Term *)
 | TmBind : Term -> Term -> Term
-| TmIf : Term -> Term -> Term -> Term
-| TmTable : Ty -> Term.
+(* | TmIf : Term -> Term -> Term -> Term
+| TmTable : Ty -> Term *)
+.
 
 Notation "L @ M" := (TmApp L M) (at level 500).
-Notation "〈 L , M 〉" := (TmPair L M) (at level 400).
+(* Notation "〈 L , M 〉" := (TmPair L M) (at level 400). *)
 
 (** Typing derivations *)
 Inductive Typing env : Term -> Ty -> Set :=
@@ -44,34 +45,34 @@ Inductive Typing env : Term -> Ty -> Set :=
 | TVar : forall (x:nat) ty,
     value ty = nth_error env x ->
     Typing env (TmVar x) ty
-| TPair : forall l m s t, Typing env l s -> Typing env m t ->
-    Typing env (TmPair l m) (TyPair s t)
+(* | TPair : forall l m s t, Typing env l s -> Typing env m t ->
+    Typing env (TmPair l m) (TyPair s t) *)
 | TApp : forall l m a b,
     Typing env l (TyArr a b) -> Typing env m a ->
     Typing env (TmApp l m) b
 | TAbs : forall n s t,
     Typing (s :: env) n t ->
     Typing env (TmAbs n) (TyArr s t)
-| TProj1 : forall m s t,
+(* | TProj1 : forall m s t, 
     Typing env m (TyPair s t) ->
     Typing env (TmProj false m) s
 | TProj2 : forall m s t,
     Typing env m (TyPair s t) ->
-    Typing env (TmProj true m) t
+    Typing env (TmProj true m) t *)
 | TSingle : forall m t,
     Typing env m t ->
     Typing env (TmSingle m) (TyList t)
-| TUnion : forall m n t,
+(* | TUnion : forall m n t,
     Typing env m (TyList t) ->
     Typing env n (TyList t) ->
     Typing env (TmUnion m n) (TyList t)
 | TNull : forall t,
-    Typing env TmNull (TyList t)
+    Typing env TmNull (TyList t) *)
 | TBind : forall m s n t,
     Typing env m (TyList s) ->
     Typing (s::env) n (TyList t) ->
     Typing env (TmBind m n) (TyList t)
-| TTable : forall r, Typing env (TmTable r) (TyList r)
+(* | TTable : forall r, Typing env (TmTable r) (TyList r) *)
 .
 
 #[export]
@@ -146,20 +147,20 @@ Fixpoint freevars (M:Term) : set nat :=
   match M with
   | TmConst => empty_set nat
   | TmVar x => set_add eq_nat_dec x (empty_set nat)
-  | TmPair L M => set_union eq_nat_dec (freevars L) (freevars M)
-  | TmProj b M => freevars M
+  (* | TmPair L M => set_union eq_nat_dec (freevars L) (freevars M) *)
+  (* | TmProj b M => freevars M *)
   | TmAbs N => set_map eq_nat_dec pred
                  (set_remove _ eq_nat_dec 0 (freevars N))
   | TmApp L M => set_union eq_nat_dec (freevars L) (freevars M)
-  | TmNull => empty_set nat
+  (* | TmNull => empty_set nat *)
   | TmSingle x => freevars x
-  | TmUnion a b => set_union eq_nat_dec (freevars a) (freevars b)
+  (* | TmUnion a b => set_union eq_nat_dec (freevars a) (freevars b) *)
   | TmBind M N => set_union eq_nat_dec (freevars M)
                             (set_map eq_nat_dec pred
                                      (set_remove _ eq_nat_dec 0 (freevars N)))
-  | TmIf b M N => set_union eq_nat_dec (freevars b)
+  (* | TmIf b M N => set_union eq_nat_dec (freevars b)
                             (set_union eq_nat_dec (freevars M) (freevars N))
-  | TmTable _ => empty_set nat
+  | TmTable _ => empty_set nat *)
   end.
 
 Definition free_in x M := set_In x (freevars M).
@@ -168,7 +169,6 @@ Definition in_env_domain (n:nat) (env:list Term) := fun x => n <= x < n+length e
 (* (* Alt definition, reuses outside_range; consider it! *)
    Definition in_env_domain (n:nat) (env:list Term) :=
    fun x => false = outside_range n (n+length env) x. *)
-
 
 (* TODO: in_env_domain and outside_range are essentially logical inverses,
    but are defined in different sorts. Consolidate them! *)
@@ -191,14 +191,19 @@ Qed.
     TODO: Fix that!
  *)
 Inductive Neutral : Term -> Type :=
+  | Neutral_Var : forall x, Neutral (TmVar x)
   | Neutral_App : forall L M, Neutral (TmApp L M)
-  | Neutral_Proj : forall b M, Neutral (TmProj b M)
-  | Neutral_Table : forall t, Neutral (TmTable t).
+  (* | Neutral_Proj : forall b M, Neutral (TmProj b M)
+  | Neutral_Table : forall t, Neutral (TmTable t) *)
+  .
 
 #[export]
 Hint Constructors Neutral.
 
 #[export]
 Hint Resolve Neutral_App.
+Hint Resolve Neutral_Var.
 #[export]
-Hint Resolve Neutral_Proj.
+Hint Resolve Neutral_App.
+(* #[export] *)
+(* Hint Resolve Neutral_Proj. *)
